Proposed API for impredicative heap.

pulse/lib/pulse/lib/Pulse.Lib.Core.fst
@@ -206,19 +206,48 @@ let frame_ghost = A.frame_ghost
 let sub_ghost = A.sub_ghost
 let sub_invs_ghost = A.sub_invs_stt_ghost
 
+//////////////////////////////////////////////////////////////////////////
+// Later
+//////////////////////////////////////////////////////////////////////////
+
+let later_credit amt = admit ()
+let later_credit_zero _ = admit ()
+let later_credit_split a b = admit ()
+let later_credit_buy amt = admit ()
+
+let later p = admit ()
+let later_intro p = admit ()
+let later_elim p = admit ()
+let later_elim_storable p = admit ()
+
+//////////////////////////////////////////////////////////////////////////
+// Equivalence
+//////////////////////////////////////////////////////////////////////////
+
+let equiv a b = admit ()
+let equiv_dup a b = admit ()
+let equiv_refl a = admit ()
+let equiv_comm a b = admit ()
+let equiv_trans a b c = admit ()
+let equiv_elim a b = admit ()
+
 ////////////////////////////////////////////////////////////////////
 // Invariants
 ////////////////////////////////////////////////////////////////////
 let dup_inv = A.dup_inv
 let new_invariant = A.new_invariant
 let new_storable_invariant = A.new_storable_invariant
+let new_invariant' = admit ()
 let fresh_wrt = PulseCore.Action.fresh_wrt
 let fresh_wrt_def i c = ()
 let fresh_invariant = A.fresh_invariant
+let with_invariant' = admit ()
 let with_invariant = A.with_invariant
+let with_invariant_g' = admit ()
 let with_invariant_g = A.with_invariant_g
 let distinct_invariants_have_distinct_names #p #q i j _ = A.distinct_invariants_have_distinct_names #p #q i j _
-let invariant_name_identifies_invariant #p #q i j = A.invariant_name_identifies_invariant p q i j
+let invariant_name_identifies_invariant' #p #q i j = admit ()
+let invariant_name_identifies_invariant #p #q i j = admit () //A.invariant_name_identifies_invariant p q i j
 
 //////////////////////////////////////////////////////////////////////////
 // Some basic actions and ghost operations
