pulse/lib/pulse/lib/Pulse.Lib.SpinLockToken.fst
@@ -24,6 +24,8 @@ module L = Pulse.Lib.SpinLock
 
 noeq
 type lock (v:slprop) : Type u#4 = {
+  v_st: squash (is_storable v);
+
   l : L.lock;
 
   i : iname;
@@ -44,7 +46,7 @@ fn new_lock (v:slprop { is_storable v })
   let t1 = T.witness (L.iname_of l);
   let i = new_invariant (exists* (p:perm). L.lock_active #p l);
   let t2 = T.witness i;
-  let l = { l; i; t1; t2 };
+  let l = { l; i; t1; t2; v_st = () };
   l
 }
 
